\documentclass[12pt,border=4pt,multi]{article} % \documentclass[tikz,border=4pt,multi]{article}
\usepackage{lingmacros}
\usepackage{tree-dvips}
\usepackage{amssymb} % for mathbb{}
\usepackage[dvipsnames]{xcolor}
\usepackage{forest}
\usepackage{amsmath} % for matrices
\usepackage{xeCJK}
\usepackage{tikz}
\usepackage[arrowdel]{physics}
\usepackage{graphicx}
\usepackage{wrapfig}
\usepackage{listings}
\usepackage{pgfplots, pgfplotstable}
\usepackage{diagbox} % diagonal line in cell
\usepackage[usestackEOL]{stackengine}
\usepackage{multirow}
\graphicspath{{./img}} % specify the graphics path to be relative to the main .tex file, denoting the main .tex file directory as ./
\newcommand\Myperm[2][^n]{\prescript{#1\mkern-2.5mu}{}P_{#2}}
\newcommand\Mycomb[2][^n]{\prescript{#1\mkern-0.5mu}{}C_{#2}}
\definecolor{orchid}{rgb}{0.7, 0.4, 1.1}

\begin{document}

\section*{Xi Liu, xl3504, Problem Set 8}
Problem 1\\
\begin{align*}
Cov(X, Y) &= E[XY] - E[X]E[Y]
\end{align*}
\begin{align*}
E[g(X, Y)] &= \sum_i \sum_j g(a_i, b_j) P(X = a_i, Y = b_j)\\
g(x, y) &= xy\\
E[XY] &= \sum_i \sum_j a_i b_j P(X = a_i, Y = b_j)\\
&= (0)(100)(0.2) + (100)(100)(0.1) + (200)(100)(0.2)\\
&\quad+ (0)(250)(0.05) + (100)(250)(0.15) + (200)(250)(0.3)\\
&= 23750\\
\end{align*}
\begin{align*}
E[X] &= \sum_i a_i P(X = a_i)\\
&= (0)(0.2 + 0.05) + (100)(0.1 + 0.15) + (200)(0.2 + 0.3)\\
&= 125\\
\end{align*}
\begin{align*}
E[Y] &= \sum_j b_j P(Y = b_j)\\
&= (100)(0.2 + 0.1 + 0.2) + (250)(0.05 + 0.15 + 0.3)\\
&= 175\\
\end{align*}
\begin{align*}
Cov(X, Y) &= E[XY] - E[X]E[Y]\\
&= 23750 - (125)(175)\\
&= \boxed{1875}\\
\end{align*}
\begin{align*}
\rho(X, Y) &= \frac{Cov(X, Y)}{\sqrt{Var(X) Var(Y)}}
\end{align*}
\begin{align*}
Var(X) &= E[X^2] - E[X]^2\\
\end{align*}
\begin{align*}
E[g(X)] &= \sum_i g(a_i) P(X = a_i)\\
g(x) &= x^2\\
E[X^2] &= \sum_i a_i^2 P(X = a_i)\\
&= (0)^2(0.2 + 0.05) + (100)^2(0.1 + 0.15) + (200)^2(0.2 + 0.3)\\
&= 22500\\
\end{align*} 
\begin{align*}
Var(X) &= E[X^2] - E[X]^2\\
&= 22500 - (125)^2\\
&= 6875\\
\end{align*}
\begin{align*}
Var(Y) &= E[Y^2] - E[Y]^2\\
\end{align*}
\begin{align*}
E[g(Y)] &= \sum_j g(b_j) P(Y = b_j)\\
g(y) &= y^2\\
E[Y^2] &= \sum_j b_j^2 P(Y = b_j)\\
&= (100)^2(0.2 + 0.1 + 0.2) + (250)^2(0.05 + 0.15 + 0.3)\\
&= 36250\\
\end{align*} 
\begin{align*}
Var(Y) &= E[Y^2] - E[Y]^2\\
&= 36250 - (175)^2\\
&= 5625\\
\end{align*}
\begin{align*}
\rho(X, Y) &= \frac{Cov(X, Y)}{\sqrt{Var(X) Var(Y)}}\\
&= \frac{1875}{\sqrt{(6875)(5625)}}\\
&= \frac{1875}{1875\sqrt{11}}\\
&= \frac{1}{\sqrt{11}}\\
&= \boxed{\frac{\sqrt{11}}{11}}\\
\end{align*}
\newpage
\noindent
Problem 2\\
1.\\
let $area$ be the area of triangle\\
\begin{center}
$\exists a \in \mathbb{R}$\\
$f_{X, Y}(x, y) = 
\begin{cases}
a & \text{if}\;(x, y) \in T\\
0 & \text{otherwise}\\
\end{cases}$
\end{center}
\begin{align*}
1 &= \int_0^1 \int_0^{1 - x} f_{X, Y}(x, y) dy dx\\
&= \int_0^1 \int_0^{1 - x} a\; dy dx\\
&= \int_0^1 [ay]_{y = 0}^{y = 1 - x} dx\\
&= \int_0^1 a(1 - x)dx\\
&= a\left[x - \frac{x^2}{2}\right]_0^1\\
&= a\left[1 - \frac{1}{2}\right]\\
&= \frac{a}{2}\\
\end{align*}
\begin{align*}
1 &= \frac{a}{2}\\
a &= 2\\
\end{align*}
alternatively
\begin{align*}
area &= \frac{(1 - 0)(1 - 0)}{2} = \frac{1}{2}\\
a &= \frac{1}{area} = \frac{1}{1 / 2} = 2\\
\end{align*}
\begin{center}
$\boxed{f_{X, Y}(x, y) = 
\begin{cases}
2 & \text{if}\; 0 \leq x \leq 1,\; 0 \leq y \leq 1\\
0 & \text{otherwise}\\
\end{cases}}$
\end{center}
\leavevmode
\\
\\
\\
\\
\\
2.
\begin{align*}
f_X(x) &= \int_{-\infty}^{\infty} f_{X, Y}(x, y) dy\\
&= \int_{0}^{1 - x} 2 dy\\
&= [2y]_0^{1 - x}\\
&= 2(1 - x)\\
&= 2 - 2x\\
\end{align*}
\begin{center}
$\boxed{f_X(x) =
\begin{cases}
2 - 2x & \text{if } 0 \leq x \leq 1\\
0 & \text{otherwise}\\
\end{cases}}$
\end{center}
\begin{align*}
f_Y(y) &= \int_{-\infty}^{\infty} f_{X, Y}(x, y) dx\\
&= \int_{0}^{1 - y} 2 dx\\
&= [2x]_0^{1 - y}\\
&= 2(1 - y)\\
&= 2 - 2y\\
\end{align*}
\begin{center}
$\boxed{f_Y(y) =
\begin{cases}
2 - 2y & \text{if } 0 \leq y \leq 1\\
0 & \text{otherwise}\\
\end{cases}}$
\end{center}
\leavevmode
\\
\\
\\
\\
\\
3.
\begin{align*}
f_{X}(x)f_{Y}(y) &= (2 - 2x)(2 - 2y)\\
&= 4 - 4y - 4x + 4xy\\
f_{X, Y}(x, y) = 2 &\not= f_{X}(x)f_{Y}(y) = 4 - 4y - 4x + 4xy
\end{align*}
for example if $x = 0$, $y = 0$, $f_{X}(x)f_{Y}(y) = 4 \not= f_{X, Y}(x, y) = 2$\\
so $X$ and $Y$ are not independent random variables\\
\\
\\
\\
\\
4.
\begin{align*}
Cov(X, Y) &= E[XY] - E[X]E[Y]\\
\end{align*}
\begin{align*}
E[g(X, Y)] &= \int_{-\infty}^{\infty} \int_{-\infty}^{\infty} g(x, y) f_{X, Y}(x, y) dx dy\\
g(x, y) &= xy;\quad 0 \leq x \leq 1 - y;\quad 0 \leq y \leq 1,\quad f_{X, Y}(x, y) = 2\\
E[XY] &= 2\int_{0}^{1} \int_{0}^{1 - y} xy\; dx dy\\
&= 2\int_{0}^{1} \left[\frac{x^2y}{2}\right]_{x = 0}^{x = 1 - y} dy\\
&= \int_{0}^{1} (1 - y)^2y dy\\
&= \int_{0}^{1} (1 - 2y + y^2)y dy\\
&= \int_{0}^{1} (y - 2y^2 + y^3) dy\\
&= \left[\frac{y}{2} - \frac{1}{3}y^3 + \frac{1}{4}y^4\right]_0^1\\
&= \frac{1}{2} - \frac{2}{3} + \frac{1}{4}\\
&= \frac{1}{12}\\
\end{align*}
\begin{align*}
E[X] &= \int_{-\infty}^{\infty} x f_X(x) dx\\
f_X(x) &= 2 - 2x;\quad 0 \leq x \leq 1\\
E[X] &= \int_{0}^{1} x(2 - 2x)\;dx\\
&= \int_{0}^{1} (2x - 2x^2)\;dx\\
&= \left[x^2 - \frac{2}{3}x^3\right]_0^1\\
&= \frac{1}{3}\\
\end{align*}
\begin{align*}
E[Y] &= \int_{-\infty}^{\infty} y f_Y(y) dy\\
f_Y(y) &= 2 - 2y;\quad 0 \leq y \leq 1\\
E[Y] &= \int_{0}^{1} y(2 - 2y)\;dy\\
&= \int_{0}^{1} (2y - 2y^2)\;dy\\
&= \left[y^2 - \frac{2}{3}y^3\right]_0^1\\
&= \frac{1}{3}\\
\end{align*}
\begin{align*}
Cov(X, Y) &= E[XY] - E[X]E[Y]\\
&= \frac{1}{12} - \frac{1}{3} \cdot \frac{1}{3}\\
&= \boxed{-\frac{1}{36}}\\
\end{align*}
\newpage
\noindent
Problem 3\\
1.\\
since there is no replacement, $x = y$ is not possible
\begin{align*}
p_Z(z) &= P(Z = z)\\
&= \sum_{x < y} P(Z = z) + \sum_{x > y} P(Z = z)\\
&= \sum_{x = 1}^{n - z} \left(\frac{1}{n}\right)\left(\frac{1}{n - 1}\right)
+ \sum_{y = 1}^{n - z} \left(\frac{1}{n}\right)\left(\frac{1}{n - 1}\right)\\
&= \frac{n - z - 1 + 1}{n(n - 1)} + \frac{n - z - 1 + 1}{n(n - 1)}\\
&= \frac{2n - 2z}{n(n - 1)}\\
\end{align*}
\[\boxed{P(Z = z) = \frac{2n - 2z}{n(n - 1)} \quad \text{if } z \in [1, n - 1] \cap \mathbb{N}}\]
\\
\\
\\
2.
\begin{align*}
E[Z] &= \sum_{z = 1}^{n - 1} z P(Z = z)\\
&= \sum_{z = 1}^{n - 1} z \left(\frac{2n - 2z}{n(n - 1)}\right)\\
&= \sum_{z = 1}^{n - 1} \frac{2nz - 2z^2}{n(n - 1)}\\
&= \left(\frac{2n}{n(n - 1)} \sum_{z = 1}^{n - 1} z\right) - \left(\frac{2}{n(n - 1)} \sum_{z = 1}^{n - 1} z^2\right)\\
&\text{/* } \sum_{i = 1}^n i = \frac{n(n + 1)}{2};\quad \sum_{i = 1}^n i^2 = \frac{n(n + 1)(2n + 1)}{6}\text{ */}\\
&= \frac{2n}{n(n - 1)} \cdot \frac{(n - 1)((n - 1) + 1)}{2}\\
&\quad- \frac{2}{n(n - 1)} \cdot \frac{(n - 1)((n - 1) + 1)(2(n - 1) + 1)}{6}\\
&= \frac{2}{n - 1} \cdot \frac{n(n - 1)}{2} - \frac{2}{n(n - 1)} \cdot \frac{n(n - 1)(2n - 1)}{6}\\
&= \boxed{n - \frac{2n - 1}{3}}\\
\end{align*}
\newpage
\noindent
Problem 4\\
1.\\
let $N_{[x, t]}$ be the total number of arrivals in the interval $[x, t]$ for the Poisson process
\begin{align*}
P(N_{[x, t]} = k) = \frac{(\lambda (t - x))^k}{k!} e^{-\lambda (t - x)}\\
\end{align*}
\begin{align*}
P(N_{(3, 8]} = 0) &= \frac{(0.5(8 - 3))^0}{0!} e^{-0.5 (8 - 3)}\\
&= \boxed{e^{-5 / 2}}\\
\end{align*}
\\
\\
\\
\\
2.
\begin{align*}
P(N_{(0, 1]} = 1) &= \frac{(0.5(1 - 0))^1}{1!} e^{-0.5(1 - 0)}\\
&= \frac{1}{2}e^{-1 / 2}\\
\end{align*}
\begin{align*}
P(N_{(1, 2]} = 1) &= \frac{(0.5(2 - 1))^1}{1!} e^{-0.5(2 - 1)}\\
&= \frac{1}{2}e^{-1 / 2}\\
\end{align*}
\begin{align*}
P(N_{(2, 3]} = 1) &= \frac{(0.5(3 - 2))^1}{1!} e^{-0.5(3 - 2)}\\
&= \frac{1}{2}e^{-1 / 2}\\
\end{align*}
\begin{align*}
P(N_{(3, 4]} = 1) &= \frac{(0.5(4 - 3))^1}{1!} e^{-0.5(4 - 3)}\\
&= \frac{1}{2}e^{-1 / 2}\\
\end{align*}
since the 4 time intervals are disjoint 
\begin{align*}
&P(N_{(0, 1]} = 1, N_{(1, 2]} = 1, N_{(2, 3]} = 1, N_{(3, 4]} = 1)\\
&= P(N_{(0, 1]} = 1)P(N_{(1, 2]} = 1)P(N_{(2, 3]} = 1)P(N_{(3, 4]} = 1)\\
&= \boxed{\left(\frac{1}{2}e^{-1 / 2}\right)^4}\\
&= \boxed{\frac{1}{16}e^{-2}}\\
\end{align*}
\newpage
\noindent
Problem 5
\begin{align*}
Cov(N_{t_1}, N_{t_2}) = E[N_{t_1}N_{t_2}] - E[N_{t_1}]E[N_{t_2}]
\end{align*}
\begin{align*}
P(N_{t_1} = k) &= \frac{(\lambda t_1)^k}{k!} e^{-\lambda t_1}\\
P(N_{t_2} = k) &= \frac{(\lambda t_2)^k}{k!} e^{-\lambda t_2}\\
E[N_{t_1}] &= \lambda t_1\\
E[N_{t_2}] &= \lambda t_2\\
Var(N_{t_1}) &= \lambda t_1\\
\end{align*}
\begin{align*}
E[N_{t_1} N_{t_2}] &= E[N_{t_1}(N_{t_2} - N_{t_1} + N_{t_1})]\\
&= E[N_{t_1}(N_{t_2} - N_{t_1}) + N_{t_1}^2]\\
&= E[N_{t_1}(N_{t_2} - N_{t_1})] + E[N_{t_1}^2]\\
&\text{/* since $(0, t_1]$ and $(t_1, t_2]$ are disjoint time intervals,}\\
&\text{$N_{t_1}$ and $N_{t_2} - N_{t_1}$ are independent random variables */}\\
&= E[N_{t_1}]E[N_{t_2} - N_{t_1}] + E[N_{t_1}^2]\\
\end{align*}
\begin{align*}
Var(N_{t_1}) &= E[N_{t_1}^2] - E[N_{t_1}]^2\\
\\
E[N_{t_1}^2] &= Var(N_{t_1}) + E[N_{t_1}]^2\\
&= \lambda t_1 + (\lambda t_1)^2\\
\end{align*}
\\
\begin{align*}
E[N_{t_1} N_{t_2}] &= E[N_{t_1}]E[N_{t_2} - N_{t_1}] + E[N_{t_1}^2]\\
&= (\lambda t_1)(\lambda (t_2 - t_1)) + (\lambda t_1 + (\lambda t_1)^2)\\
&= (\lambda t_1)(\lambda (t_2 - t_1)) + \lambda t_1 + (\lambda t_1)^2\\
&= \lambda^2 t_1 t_2 - \lambda^2 t_1^2 + \lambda t_1 + \lambda^2 t_1^2\\
&= \lambda^2 t_1 t_2 + \lambda t_1\\
\end{align*}
\begin{align*}
Cov(N_{t_1}, N_{t_2}) &= E[N_{t_1}N_{t_2}] - E[N_{t_1}]E[N_{t_2}]\\
&= \lambda^2 t_1 t_2 + \lambda t_1 - (\lambda t_1)(\lambda t_2)\\
&= \lambda^2 t_1 t_2 + \lambda t_1 - \lambda^2 t_1 t_2\\
&= \boxed{\lambda t_1}\\
\end{align*}
\end{document}